Simu/Sep.v
@@ -129,6 +129,31 @@ Section Sepall.
     intro p. apply sepall_breakout with (1:=Hys).
   Qed.
 
+  Lemma sepall_in_map:
+    forall x ys f,
+      In x (map f ys) ->
+      exists x' ws xs,
+        x = f x' 
+        /\ ys = ws ++ x' :: xs
+        /\ (forall p,
+              sepall p ys <-*-> p x ** sepall p (ws ++ xs)).
+  Proof.
+    intros x ys f Hin.
+    apply in_split in Hin.
+    destruct Hin as [ws [xs Hys]].
+    pose proof Hys as Hys'. 
+    apply map_app' in Hys'.
+    destruct Hys' as (ws' & xxs' & Hws & Hxxs).
+    symmetry in Hxxs.
+    apply map_cons' in Hxxs.
+    destruct Hxxs as (x' & xs' & Hx & Hxs).
+    subst.
+    exists x' ws' xs'.
+    splits*; auto. 
+    - admit.
+    - intro p. admit.
+  Qed.
+
   Lemma sepall_sepfalse:
     forall m p xs,
       m |= sepall p xs ->
@@ -270,8 +295,6 @@ Section SplitRange.
 
 End SplitRange.
 
-Definition chunk_of_type ty := AST.chunk_of_type (Ctypes.typ_of_type ty).
-
 Definition match_value (e: PM.t val) (x: ident) (v': val) : Prop :=
   match PM.find x e with
   | None => True
@@ -280,6 +303,26 @@ Definition match_value (e: PM.t val) (x: ident) (v': val) : Prop :=
 
 Definition match_var (S: state) :=
   match_value (snd S).
+
+Remark match_find_var_det:
+  forall S x v1 v2,
+    match_var S x v1 ->
+    find_var S x v2 ->
+    v1 = v2.
+Proof.
+  unfold match_var, match_value, find_var.
+  introv Hm Hf.
+  destruct (PM.find x (snd S)).
+  - subst; inverts* Hf.
+  - discriminate.
+Qed.
+
+Ltac app_match_find_var_det :=
+  match goal with
+  | H1: find_var ?S ?x ?v1,
+        H2: match_var ?S ?x ?v2 |- _ =>
+    assert (v2 = v1) by (applys* match_find_var_det H2 H1); subst v1; clear H2 
+  end.
 
 Definition match_field (S: state) :=
   match_value (fst S).(mm_values).
@@ -345,9 +388,9 @@ Section Staterep.
     end.
 
    Lemma staterep_skip_cons:
-    forall cls prog clsnm me b ofs,
+    forall cls prog clsnm S b ofs,
       clsnm <> cls.(c_name) ->
-      staterep (cls :: prog) clsnm me b ofs <-*-> staterep prog clsnm me b ofs.
+      staterep (cls :: prog) clsnm S b ofs <-*-> staterep prog clsnm S b ofs.
   Proof.
     intros ** Hnm.
     apply ident_eqb_neq in Hnm.
@@ -355,9 +398,9 @@ Section Staterep.
   Qed.
 
   Lemma staterep_skip_app:
-    forall clsnm prog oprog me b ofs,
+    forall clsnm prog oprog S b ofs,
       ~ClassIn clsnm oprog ->
-      staterep (oprog ++ prog) clsnm me b ofs <-*-> staterep prog clsnm me b ofs.
+      staterep (oprog ++ prog) clsnm S b ofs <-*-> staterep prog clsnm S b ofs.
   Proof.
     intros ** Hnin.
     induction oprog as [|cls oprog IH].
@@ -366,22 +409,8 @@ Section Staterep.
       rewrite <-app_comm_cons.
       rewrite staterep_skip_cons; auto.
   Qed.
-
-End Staterep.
-
-Section BlockRep.
-  Variable ge : composite_env.
-
-  Definition blockrep (S: state) (flds: members) (b: block) : massert :=
-    sepall (fun xty : ident * type =>
-              let (x, ty) := xty in
-              match field_offset ge x flds, access_mode ty with
-              | OK d, By_value chunk =>
-                contains chunk b d (match_var S x)
-              | _, _ => sepfalse
-              end) flds.
   
-End BlockRep.
+End Staterep.
 
 Lemma ident_eqb_sym:
   forall x y, ident_eqb x y = ident_eqb y x.
@@ -469,11 +498,6 @@ Proof.
       apply NotInMembers_NotIn in Heq; intuition.
 Qed.
 
-Definition valid_val (v: val) (t: typ): Prop :=
-    Ctypes.access_mode t = Ctypes.By_value (chunk_of_type t)
-    /\ v <> Values.Vundef
-    /\ Values.Val.has_type v (Ctypes.typ_of_type t).
-
 Lemma sizeof_translate_chunk:
   forall gcenv t,
     Ctypes.access_mode t = Ctypes.By_value (chunk_of_type t) ->
@@ -508,3 +532,433 @@ Proof.
   split*.
   now apply align_chunk_divides_alignof_type.  
 Qed.
+
+Section StateRepProperties.
+
+  Variable main_node : ident.
+  Variable prog: program.
+  Variable tprog: Clight.program.
+   
+  Let tge := Clight.globalenv tprog.
+  Let gcenv := Clight.genv_cenv tge.
+  
+  Definition pointer_of_node node := pointer_of (type_of_inst node).
+
+  Hypothesis TRANSL: translate prog main_node = Errors.OK tprog.
+  Hypothesis main_node_exists: find_class main_node prog <> None.
+ 
+  Lemma make_members_co:
+    forall clsnm cls prog',
+      find_class clsnm prog = Some (cls, prog') ->
+      (exists co, gcenv!clsnm = Some co
+             /\ co_su co = Struct
+             /\ co_members co = make_members cls
+             /\ attr_alignas (co_attr co) = None
+             /\ NoDupMembers (co_members co)).
+  Proof.
+    unfold translate in TRANSL.
+    apply not_None_is_Some in main_node_exists.
+    destruct main_node_exists as [[maincls prog'] Hfind_main].
+    rewrite Hfind_main in TRANSL.
+    destruct (map (translate_class prog) prog) as [|cls clss] eqn:Hmap.
+    - apply map_eq_nil in Hmap.
+      rewrite Hmap in Hfind_main; simpl in *; discriminate.
+    -
+  Admitted.
+
+  Lemma field_translate_mem_type:
+    forall clsnm cls prog',
+      find_class clsnm prog = Some (cls, prog') ->
+      NoDupMembers (make_members cls) ->
+      forall x ty,
+        In (x, ty) cls.(c_mems) ->
+        field_type x (make_members cls) = OK ty.
+  Proof.
+    introv Hfind Hndup Hin.
+    apply in_field_type with (1:=Hndup).
+    unfold make_members. apply in_app_iff. now left.
+  Qed.
+
+  Lemma field_translate_obj_type:
+    forall clsnm cls prog',
+      find_class clsnm prog = Some (cls, prog') ->
+      NoDupMembers (make_members cls) ->
+      forall o c,
+        In (o, c) cls.(c_objs) ->
+        field_type o (make_members cls) = OK (type_of_inst c).
+  Proof.
+    introv Hfind Hndup Hin.
+    apply in_field_type with (1:=Hndup).
+    unfold make_members. apply in_app_iff. right.
+    apply in_map_iff. exists* (o, c).
+  Qed.
+
+  (* TODO: Construct a global environment of structs for a given program. *)
+
+  Lemma gcenv_consistent:
+    composite_env_consistent gcenv.
+  Admitted.
+  
+  Lemma range_staterep:
+    forall ve b clsnm,
+      WelldefClasses prog ->
+      find_class clsnm prog <> None ->
+      range b 0 (sizeof gcenv (type_of_inst clsnm)) -*>
+            staterep gcenv prog clsnm (m_empty, ve) b 0.
+  Proof.
+    introv Hwdef Hfind.
+    cut (forall lo,
+           (alignof gcenv (type_of_inst clsnm) | lo) ->
+           massert_imp (range b lo (lo + sizeof gcenv (type_of_inst clsnm)))
+                       (staterep gcenv prog clsnm (m_empty, ve) b lo)).
+    - intro HH; apply HH; apply Z.divide_0_r.
+    - clear main_node_exists TRANSL.
+
+      revert clsnm Hfind.
+      induction prog as [|cls prog' IH]; intros clsnm Hfind lo.
+      + apply not_None_is_Some in Hfind.
+        destruct Hfind. discriminate.
+      + intro Halign.
+        inversion Hwdef as [|? ? Hwdef']; subst.
+
+        assert (find_class clsnm prog = Some (cls, prog')) as Hprog.
+        admit.
+        (* TODO: need to link prog to (possibly reversed) translation *)
+
+        pose proof (make_members_co _ _ _ Hprog) as Hmco.
+        destruct Hmco as [co [Hg [Hsu [Hmem [Hattr Hndup]]]]].
+
+        pose proof (co_members_alignof _ _ (gcenv_consistent _ _ Hg) Hattr)
+          as Hcoal.
+        rewrite Hmem in Hcoal.
+        unfold make_members in Hcoal.
+        apply Forall_app in Hcoal.
+        destruct Hcoal as [Hcoal1 Hcoal2].
+        simpl in Halign.
+        rewrite Hg in Halign.
+        rewrite align_noattr in Halign.
+        assert (Hndup':=Hndup). rewrite Hmem in Hndup'.
+
+        simpl.
+        destruct (ident_eqb clsnm cls.(c_name)) eqn:Hclsnm.
+        *{ rewrite Hg.
+           rewrite <-Hmem.
+           rewrite split_range_fields
+           with (1:=gcenv_consistent) (2:=Hg) (3:=Hsu) (4:=Hndup).
+           rewrite Hmem at 1.
+           unfold make_members.
+           rewrite sepall_app.
+           
+           apply sep_imp'.
+
+           - pose proof (field_translate_mem_type _ _ _ Hprog Hndup') as Htype.
+             clear Hcoal2.
+             
+             induction (c_mems cls); auto.
+             apply Forall_cons2 in Hcoal1.
+             destruct Hcoal1 as [Hcoal1 Hcoal2].
+
+             apply sep_imp'.
+             + destruct a.
+               destruct (field_offset gcenv i (co_members co)) eqn:Hfo; auto.
+               unfold match_field.
+               rewrite match_value_empty.
+               rewrite sizeof_translate_chunk.
+               *{ apply range_contains'.
+                  specialize (Htype i t).
+                  rewrite <-Hmem in Htype.
+                  apply field_offset_aligned with (ty:=t) in Hfo.
+                  - simpl in Hcoal1.
+                    apply Z.divide_add_r.
+                    + apply Zdivide_trans with (2:=Halign).
+                      apply Zdivide_trans with (2:=Hcoal1).
+                      apply align_chunk_divides_alignof_type.
+                      admit.
+                    + apply Zdivide_trans with (2:=Hfo).
+                      apply align_chunk_divides_alignof_type.
+                      admit.
+                  - apply Htype; constructor; reflexivity.
+                }
+               * admit.
+             + apply IHl.
+               * apply Hcoal2.
+               * intros; apply Htype; constructor (assumption).
+         
+           - pose proof (field_translate_obj_type _ _ _ Hprog Hndup') as Htype.
+             rewrite <-Hmem in Htype.
+           
+             induction (c_objs cls); auto.
+             simpl.
+             apply sep_imp'.
+             + clear IHl.
+               
+               destruct a as [o c].
+               assert (ClassIn c prog') as Hcin
+                   by (eapply H0; econstructor; eauto).
+               clear H0 Hcoal1.
+
+               apply Forall_cons2 in Hcoal2.
+               destruct Hcoal2 as [Hcoal2 Hcoal3].
+               
+               specialize (Htype o c (in_eq _ _)).
+               clear Hcoal3 l.
+
+               simpl.
+               destruct (field_offset gcenv o (co_members co)) eqn:Hfo; auto.
+               rewrite instance_match_empty.
+               apply ClassIn_find_class in Hcin.
+               specialize (IH Hwdef' c Hcin (lo + z)%Z).
+
+               apply not_None_is_Some in Hcin.
+               destruct Hcin as ((c' & prog'') & Hcin).
+               assert (find_class c prog = Some (c', prog'')) as Hcin'.
+               admit. (* TODO: make_members_co should be more flexible. *)
+
+               assert (Hcin'' := Hcin').
+               apply make_members_co in Hcin'.
+               destruct Hcin' as [? [? [? [? [? ?]]]]].
+               rewrite H.
+
+               simpl in IH.
+               rewrite H in IH.
+               apply IH.
+
+               simpl in Hcoal2.
+               rewrite align_noattr in Hcoal2.
+               rewrite H in Hcoal2.
+               
+               rewrite align_noattr.
+               apply Z.divide_add_r.
+               * apply Zdivide_trans with (1:=Hcoal2).
+                 assumption.
+
+               * simpl in Htype.
+                 eapply field_offset_aligned in Hfo.
+                 2:apply Htype.
+                 apply Zdivide_trans with (2:=Hfo).
+                 simpl. rewrite H, align_noattr.
+                 apply Z.divide_refl.
+             + apply IHl.
+               * clear IHl. intros o c' Hin.
+                 apply H0 with (o:=o). constructor (assumption).
+               * simpl in Hcoal2. apply Forall_cons2 in Hcoal2.
+               destruct Hcoal2 as [Hcoal2 Hcoal3]. exact Hcoal3.
+               * intros o c Hin. apply Htype. constructor (assumption).
+         }
+
+        * rewrite Hg.
+          simpl in Hfind.
+          rewrite ident_eqb_sym in Hclsnm.
+          rewrite Hclsnm in Hfind.
+          specialize (IH Hwdef' clsnm Hfind lo).
+          simpl in IH.
+          rewrite Hg in IH.
+          apply IH.
+          rewrite align_noattr.
+          assumption.
+  Qed.
+
+  Lemma staterep_deref_mem:
+    forall cls prog' m S b ofs x ty d v,
+      access_mode ty = By_value (chunk_of_type ty) ->
+      m |= staterep gcenv (cls::prog') cls.(c_name) S b ofs ->
+      In (x, ty) cls.(c_mems) ->
+      find_field S x v ->
+      field_offset gcenv x (make_members cls) = OK d ->
+      Clight.deref_loc ty m b (Integers.Int.repr (ofs + d)) v.
+  Proof.
+    intros ** Hty Hm Hin Hv Hoff.
+    simpl in Hm. rewrite ident_eqb_refl in Hm.
+    apply sep_proj1 in Hm.
+    apply sepall_in in Hin.
+    destruct Hin as [ws [xs [Hsplit Hin]]].
+    rewrite Hin in Hm. clear Hsplit Hin.
+    apply sep_proj1 in Hm. clear ws xs.
+    rewrite Hoff in Hm. clear Hoff.
+    apply loadv_rule in Hm.
+    destruct Hm as [v' [Hloadv Hmatch]].
+    unfold match_field, match_value in Hmatch.
+    unfold find_field, mfind_mem in Hv.
+    rewrite Hv in Hmatch. clear Hv.
+    rewrite <-Hmatch in Hloadv. clear Hmatch.
+    apply Clight.deref_loc_value with (2:=Hloadv); auto.
+  Qed.
+
+  Lemma staterep_assign_mem:
+    forall P cls prog' m m' S b ofs x ty d v,
+      access_mode ty = By_value (chunk_of_type ty) ->
+      NoDup cls.(c_objs) ->
+      NoDupMembers cls.(c_mems) ->
+      m |= staterep gcenv (cls::prog') cls.(c_name) S b ofs ** P ->
+      In (x, ty) cls.(c_mems) ->
+      field_offset gcenv x (make_members cls) = OK d ->
+      v = Values.Val.load_result (chunk_of_type ty) v ->
+      Clight.assign_loc gcenv ty m b (Integers.Int.repr (ofs + d)) v m' ->
+      m' |= staterep gcenv (cls::prog') cls.(c_name) (update_field S x v) b ofs ** P.
+  Proof.
+    Opaque sepconj.
+    intros ** Hty Hcls Hmem Hm Hin Hoff Hlr Hal.
+    simpl in *. rewrite ident_eqb_refl in *.
+    rewrite sep_assoc. rewrite sep_assoc in Hm.
+    apply sepall_in in Hin.
+    destruct Hin as [ws [xs [Hsplit Hin]]].
+    rewrite Hsplit in Hmem.
+    rewrite Hin in Hm. rewrite sep_assoc in Hm.
+    rewrite Hin. rewrite sep_assoc.
+    rewrite Hoff in *.
+    rewrite sep_swap2.
+    rewrite sepall_switchp
+    with (f':=fun xty : ident * typ =>
+                let (x0, ty0) := xty in
+                match field_offset gcenv x0 (make_members cls) with
+                | OK d0 =>
+                  contains (chunk_of_type ty0) b (ofs + d0)
+                           (match_field S x0)
+                | Error _ => sepfalse
+                end).
+    - rewrite <-sep_swap2.
+      eapply storev_rule' with (1:=Hm).
+      + unfold match_field, match_value. simpl.
+        rewrite PM.gss. exact Hlr.
+      + clear Hlr. inversion Hal as [? ? ? Haccess|? ? ? ? Haccess].
+        * rewrite Hty in Haccess.
+          injection Haccess. intro; subst. assumption.
+        * rewrite Hty in Haccess. discriminate.
+    - apply NoDupMembers_remove_1 in Hmem.
+      apply NoDupMembers_NoDup with (1:=Hmem).
+    - intros x' Hin'; destruct x' as [x' ty'].
+      unfold match_field, update_field, madd_mem; simpl.
+      rewrite match_value_add; [reflexivity|].
+      apply NoDupMembers_app_cons in Hmem.
+      destruct Hmem as [Hmem].
+      apply In_InMembers in Hin'.
+      intro Heq. apply Hmem. rewrite Heq in Hin'.
+      assumption.
+  Qed.
+
+  Lemma staterep_field_offset:
+    forall m S cls prog b ofs x ty,
+      m |= staterep gcenv (cls :: prog) cls.(c_name) S b ofs ->
+      In (x, ty) (make_members cls) ->
+      exists d, field_offset gcenv x (make_members cls) = OK d.
+  Proof.
+    introv Hm Hin.
+    simpl in Hm. rewrite ident_eqb_refl in Hm.
+    apply in_app_or in Hin.
+    destruct Hin as [Hin | Hin];
+      apply sepall_in in Hin; destruct Hin as [ws [xs [Hsplit Hin]]].      
+    - apply sep_proj1 in Hm.
+      rewrite Hin in Hm. clear Hsplit Hin.
+      apply sep_proj1 in Hm. clear ws xs.
+      destruct (field_offset gcenv x (make_members cls)).
+      + exists* z.
+      + contradict Hm.
+    - apply sep_proj2 in Hm.
+      admit.
+  Qed.
+  
+End StateRepProperties.
+
+Section BlockRep.
+  Variable ge : composite_env.
+
+  Definition blockrep (S: state) (flds: members) (b: block) : massert :=
+    sepall (fun xty : ident * type =>
+              let (x, ty) := xty in
+              match field_offset ge x flds, access_mode ty with
+              | OK d, By_value chunk =>
+                contains chunk b d (match_var S x)
+              | _, _ => sepfalse
+              end) flds.
+
+  Lemma blockrep_deref_mem:
+    forall m S co b x ty d v,
+      m |= blockrep S (co_members co) b ->
+      In (x, ty) (co_members co) ->
+      find_var S x v ->
+      field_offset ge x (co_members co) = OK d ->
+      Clight.deref_loc ty m b (Integers.Int.repr d) v.
+  Proof.
+    intros ** Hm Hin Hv Hoff.
+    unfold blockrep in Hm.
+    apply sepall_in in Hin.
+    destruct Hin as [ws [xs [Hsplit Hin]]].
+    rewrite Hin in Hm. clear Hsplit Hin.
+    apply sep_proj1 in Hm. clear ws xs.
+    rewrite Hoff in Hm. clear Hoff.
+    destruct (access_mode ty) eqn:Haccess; try contradiction.
+    apply loadv_rule in Hm.
+    destruct Hm as [v' [Hloadv Hmatch]].
+    unfold match_var, match_value in Hmatch.
+    unfold find_var in Hv.
+    rewrite Hv in Hmatch. clear Hv.
+    rewrite <-Hmatch in Hloadv. clear Hmatch.
+    apply Clight.deref_loc_value with (1:=Haccess) (2:=Hloadv).
+  Qed.
+
+  Lemma blockrep_assign_mem:
+    forall P co m m' S b d x v ty chunk,
+      NoDupMembers (co_members co) ->
+      m |= blockrep S (co_members co) b ** P ->
+      In (x, ty) (co_members co) ->
+      field_offset ge x (co_members co) = OK d ->
+      access_mode ty = By_value chunk ->
+      v = Val.load_result chunk v ->
+      Clight.assign_loc ge ty m b (Integers.Int.repr d) v m' ->
+      m' |= blockrep (update_var S x v) (co_members co) b ** P.
+  Proof.
+    Opaque sepconj.
+    intros ** Hndup Hm Hin Hoff Haccess Hlr Hal.
+    apply sepall_in in Hin.
+    destruct Hin as [ws [xs [Hsplit Hin]]].
+    unfold blockrep in *.
+    rewrite Hin in Hm. rewrite sep_assoc in Hm.
+    rewrite Hin. rewrite sep_assoc.
+    rewrite Hoff in *.
+    rewrite sep_swap2.
+    rewrite Haccess in *.
+    rewrite Hsplit in Hndup.
+    rewrite sepall_switchp
+    with (f':=fun xty : ident * type =>
+            let (x0, ty0) := xty in
+            match field_offset ge x0 (co_members co), access_mode ty0 with
+            | OK d0, By_value chunk =>
+              contains chunk b d0 (match_var S x0)
+            | _, _ => sepfalse
+            end).
+    - rewrite <-sep_swap2.
+      eapply storev_rule' with (1:=Hm).
+      + unfold match_var, match_value, update_var. simpl. rewrite PM.gss. exact Hlr.
+      + inversion Hal as [? ? ? Haccess'|]; rewrite Haccess in *.
+        * injection Haccess'. intro HR; rewrite <-HR in *; assumption.
+        * discriminate.
+    - apply NoDupMembers_remove_1 in Hndup.
+      apply NoDupMembers_NoDup with (1:=Hndup).
+    - intros x' Hin'; destruct x' as [x' ty'].
+      unfold match_var, update_var. simpl.
+      rewrite match_value_add; [reflexivity|].
+      apply NoDupMembers_app_cons in Hndup.
+      destruct Hndup as [Hndup].
+      apply In_InMembers in Hin'.
+      intro Heq. apply Hndup. rewrite Heq in Hin'.
+      assumption.
+  Qed.
+
+  Lemma blockrep_field_offset:
+    forall m S flds b x ty,
+      m |= blockrep S flds b ->
+      In (x, ty) flds ->
+      exists d, field_offset ge x flds = OK d.
+  Proof.
+    introv Hm Hin.
+    unfold blockrep in Hm.
+    apply sepall_in in Hin.
+    destruct Hin as [ws [xs [Hsplit Hin]]].
+    rewrite Hin in Hm. clear Hsplit Hin.
+    apply sep_proj1 in Hm. clear ws xs.
+    destruct (field_offset ge x flds).
+    - exists* z.
+    - contradict Hm.
+  Qed.
+  
+End BlockRep.
